tutorial/Imp2AsmCorrectness.v
@@ -1,3 +1,51 @@
+(** * Functional correctness of the compiler *)
+
+(** We finally turn to proving our compiler correct.
+
+    We express the result as a (weak) bisimulation between
+    the [itree] resulting from the denotation of the source
+    _Imp_ statement and the denotation of the compiled _Asm_
+    program. This weak bisimulation is a _up-to-tau_ bisimulation.
+    More specifically, we relate the itrees after having
+    interpreted the [Locals] events contained in the trees into
+    the state monad, and run them.
+
+    The proof is essentially structured as followed:
+    - a simulation relation is defined to relate the local
+    environments during the simulation. This relation is
+    strengthened into a second one used during the simulation
+    of expressions.
+    - the desired bisimulation is defined to carry out the
+    the simulation invariant into a up-to-tau after interpretation
+    of [Locals] relation. Once again a slightly different
+    bisimulation is defined when handling expressions.
+    - Linking is proved in isolation: the "high level" control
+    flow combinators for _Asm_ defined in [Imp2Asm.v] are
+    proved correct in the same style as the elemntary ones
+    from [AsmCombinators.v].
+    - Finally, all the pieces are tied together to prove the
+    correctness.
+
+    We emphasize the following aspects of the proof:
+    - Despite establishing a termination-sensitive correctness
+    result over Turing-complete languages, we have not written
+    a single [cofix]. All coinductive reasoning is internalized
+    into the [itree] library.
+    - We have separated the control-flow-related reasoning from
+    the functional correctness one. In particular, the low-level
+    [asm] combinators are entirely reusable, and the high-level
+    ones are only very loosely tied to _Imp_.
+    - All reasoning is equational. In particular, reasoning at the
+    level of [ktree]s rather than introducing the entry label and
+    trying to reason at the level of [itree]s ease sensibly the pain
+    by reducing the amount of binders under which we need to work.
+    - We transparently make use of the heterogenous bisimulation provided
+    by the [itree] library to relate computations of _Asm_ expressions
+    that return an environment and a [unit] value to ones of _Imp_
+    that return an environment and an [Imp.value].
+*)
+
+(* begin hide *)
 Require Import Imp Asm Utils_tutorial AsmCombinators Imp2Asm.
 
 Require Import Psatz.
@@ -7,18 +55,13 @@ From Coq Require Import
      Morphisms
      ZArith
      Setoid
-     Fin
      RelationClasses.
 
 From ITree Require Import
      ITree
-     Basics.Category
-     Basics.Function
-     Core.KTreeFacts
-     Effects.Env
-     Interp.MorphismsFacts
-     Interp.RecursionFacts
-     Effects.StateFacts.
+     ITreeFacts
+     Effects.StateFacts
+     Effects.Map.
 
 Import ITreeNotations.
 
@@ -35,19 +78,12 @@ Open Scope string_scope.
 Import CatNotations.
 Local Open Scope cat.
 
-Section EUTT.
+(* end hide *)
 
-  Context {E: Type -> Type}.
+(* ================================================================= *)
+(** ** Hiding mangling of variables. *)
 
-  Instance eq_itree_run_env {E R} {K V map} {Mmap: Maps.Map K V map}:
-    Proper (@eutt (envE K V +' E) R R eq ==> eq ==> @eutt E (prod map R) (prod map R) eq)
-           (run_env R).
-  Proof.
-    eapply eutt_interp_state.
-  Qed.
-
-End EUTT.
-
+(** [varOf] and [gen_tmp] are injective. *)
 Section GEN_TMP.
 
   Lemma gen_tmp_inj: forall n m, m <> n -> gen_tmp m <> gen_tmp n.
@@ -66,18 +102,47 @@ End GEN_TMP.
 Opaque gen_tmp.
 Opaque varOf.
 
+(* ================================================================= *)
+(** ** Simulation relations *)
+
+(** The compiler is proved correct by constructing a (itree) bisimulation between
+    the source program and its compilation.
+    As is traditional, we define, to this end, a simulation relation [Renv]. Since the
+    bisimulation will take place after handling of the local environment, [Renv]
+    relates two [alist var value] environments.
+ *)
+
 Section Simulation_Relation.
 
-  Variable E: Type -> Type.
-  Context {HasLocals: Locals -< E} {HasMemory: Memory -< E}.
+  (** ** Definition of the simulation relations *)
 
+  (** Relates a source variable to its mangled counterpart in _Asm_. *)
   Variant Rvar : var -> var -> Prop :=
   | Rvar_var v : Rvar (varOf v) v.
 
+  (** The simulation relation for evaluation of statements.
+      The relation relates two environments of type [alist var value].
+      The source and target environments exactly agree on user variables.
+   *)
   Definition Renv (g_asm g_imp : alist var value) : Prop :=
     forall k_asm k_imp, Rvar k_asm k_imp ->
                    forall v, alist_In k_imp g_imp v <-> alist_In k_asm g_asm v.
 
+ (** The simulation relation for evaluation of expressions.
+     The relation also relates two environments of type [alist var value],
+     but additionally the returned value at the _Imp_ level. The _Asm_
+     side does not carry a [value], but a [unit], since its denotation
+     does not return any [value].
+     The [sim_rel] relation is parameterized by the state of the [asm] environment
+     before the step, and the name of the variable used to store
+     the result.
+     It enforces three conditions:
+     - [Renv] on the environments, ensuring that evaluation of expressions
+     does not corrupt user variables;
+     - Agreement on the computed value, i.e. the returned value [v] is stored at
+     the assembly level in the expected temporary;
+     - The "stack" of temporaries used to compute intermediate results is left untouched.
+  *) 
   Definition sim_rel g_asm n: alist var value * unit -> alist var value * value -> Prop :=
     fun '(g_asm', _) '(g_imp',v) =>
       Renv g_asm' g_imp' /\            (* we don't corrupt any of the imp variables *)
@@ -85,6 +150,10 @@ Section Simulation_Relation.
       (forall m, m < n -> forall v,              (* we don't mess with anything on the "stack" *)
             alist_In (gen_tmp m) g_asm v <-> alist_In (gen_tmp m) g_asm' v).
 
+
+  (** ** Facts on the simulation relations *)
+
+  (** [Renv] is stable by updates to temporaries. *)
   Lemma Renv_add: forall g_asm g_imp n v,
       Renv g_asm g_imp -> Renv (alist_add (gen_tmp n) v g_asm) g_imp.
   Proof.
@@ -96,6 +165,7 @@ Section Simulation_Relation.
     apply In_add_ineq_iff; auto.
   Qed.
 
+  (** [Renv] entails agreement of lookup of user variables. *)
   Lemma Renv_find:
     forall g_asm g_imp x,
       Renv g_asm g_imp ->
@@ -111,6 +181,7 @@ Section Simulation_Relation.
       rewrite LUR in LUL; inv LUL.
   Qed.      
 
+  (** [sim_rel] can be initialized from [Renv]. *)
   Lemma sim_rel_add: forall g_asm g_imp n v,
       Renv g_asm g_imp ->
       sim_rel g_asm n (alist_add (gen_tmp n) v g_asm, tt) (g_imp, v).
@@ -123,6 +194,7 @@ Section Simulation_Relation.
       apply In_add_ineq_iff, gen_tmp_inj; lia.
   Qed.
 
+  (** [Renv] can be recovered from [sim_rel]. *)
   Lemma sim_rel_Renv: forall g_asm n s1 v1 s2 v2,
       sim_rel g_asm n (s1,v1) (s2,v2) -> Renv s1 s2.
   Proof.
@@ -137,6 +209,8 @@ Section Simulation_Relation.
     intros ? ? ? ? ? [_ [H _]]; exact H. 
   Qed.
 
+  (** [sim_rel] entails agreement of lookups in the "stack" between its argument
+      and the current Asm environement *)
   Lemma sim_rel_find_tmp_lt_n:
     forall g_asm n m g_asm' g_imp' v,
       m < n ->
@@ -155,15 +229,27 @@ Section Simulation_Relation.
     rewrite EQ' in EQ; easy.
   Qed.
 
-  Lemma Renv_write_local:
-    forall (x : Imp.var) (a a0 : alist var value) (v : Imp.value),
-      Renv a a0 -> Renv (alist_add (varOf x) v a) (alist_add x v a0).
+  Lemma sim_rel_find_tmp_n_trans:
+    forall g_asm n g_asm' g_asm'' g_imp' g_imp'' v v',
+      sim_rel g_asm n (g_asm', tt) (g_imp',v) ->
+      sim_rel g_asm' (S n) (g_asm'', tt) (g_imp'',v') ->
+      alist_In (gen_tmp n) g_asm'' v.
   Proof.
-    intros k m m' v.
-    repeat intro.
-    red in H.
-    specialize (H k_asm k_imp H0 v0).
-    inv H0.
+    intros.
+    generalize H; intros LU; apply sim_rel_find_tmp_n in LU.
+    unfold alist_In in LU; erewrite sim_rel_find_tmp_lt_n in LU; eauto.
+  Qed.
+
+  (** [Renv] is preserved by assignment.
+   *)
+  Lemma Renv_write_local:
+    forall (k : Imp.var) (g_asm g_imp : alist var value) v,
+      Renv g_asm g_imp ->
+      Renv (alist_add (varOf k) v g_asm) (alist_add k v g_imp).
+  Proof.
+    intros k m m' v HRel k_asm k_imp Hk v'.
+    specialize (HRel _ _ Hk v').
+    inv Hk.
     unfold alist_add, alist_In; simpl.
     do 2 flatten_goal;
       repeat match goal with
@@ -176,30 +262,84 @@ Section Simulation_Relation.
     - setoid_rewrite In_remove_In_ineq_iff; eauto using RelDec_string_Correct.
   Qed.
 
+  (** [sim_rel] can be composed when proving binary arithmetic operators. *)
+  Lemma sim_rel_binary_op:
+    forall (g_asm g_asm' g_asm'' g_imp' g_imp'' : alist var value)
+      (n v v' : nat)
+      (Hsim : sim_rel g_asm n (g_asm', tt) (g_imp', v))
+      (Hsim': sim_rel g_asm' (S n) (g_asm'', tt) (g_imp'', v'))
+      (op: nat -> nat -> nat),
+      sim_rel g_asm n (alist_add (gen_tmp n) (op v v') g_asm'', tt) (g_imp'', op v v').
+  Proof.
+    intros.
+    split; [| split].
+    {
+      eapply Renv_add, sim_rel_Renv; eassumption.
+    }
+    {
+      apply In_add_eq.
+    }
+    {
+      intros m LT v''.
+      rewrite <- In_add_ineq_iff; [| apply gen_tmp_inj; lia].
+      destruct Hsim as [_ [_ Hsim]].
+      destruct Hsim' as [_ [_ Hsim']].
+      rewrite Hsim; [| auto with arith].
+      rewrite Hsim'; [| auto with arith].
+      reflexivity.
+    }
+  Qed.
+
 End Simulation_Relation.
 
-Section Correctness.
+(* ================================================================= *)
+(** ** Bisimulation *)
+
+(** We now make precise the bisimulation established to show the correctness
+    of the compiler.
+    Naturally, we cannot establish a _strong bisimulation_ between the source
+    program and the target program: the [asm] counterpart performs "more
+    steps" when evaluating expressions.
+    The appropriate notion is of course the _equivalence up to tau_. However,
+    the [itree] structures put in evidence a very naturaly hierarchy of notions
+    of correctness.
+    Since the [asm] programs perform more manipulations of their local
+    environment, we cannot hope to relate the trees containing [Locals] events,
+    we first need to interpret them.
+    However, since it does not introduce any manipulation of the heap, we
+    _can_ prove the result without interpreting the [Memory] events.
+    Of course this example is rather contrived, owing to the simplicity of the
+    compiler. Nonetheless, it makes a lot of sense when considering optimization:
+    one can see the handling of events as bits of the memory model, and 
+    therefore have a framework to prove some optimizations correct with respect
+    to any memory model, i.e. before handling, while others with respect to
+    concrete memory model, i.e. after handling.
+ *)
+
+Section Eq_Locals.
 
   Context {E': Type -> Type}.
-  Context {HasMemory: Memory -< E'}.
-  Context {HasExit: Exit -< E'}.
   Notation E := (Locals +' E').
 
+  (** [interp_locals] handle [Locals] into the [envE] effects, and then
+      run these effects into the state monad. *)
   Definition interp_locals {R: Type} (t: itree E R) (s: alist var value)
     : itree E' (alist var value * R) :=
-    run_env _ (interp (bimap evalLocals (id_ _)) _ t) s.
+    run_map (interp (bimap evalLocals (id_ _)) t) s.
 
-  Instance eutt_interp_locals {R}:
+  (** This interpreter is compatible with the equivalence-up-to-tau. *)
+  Global Instance eutt_interp_locals {R}:
     Proper (@eutt E R R eq ==> eq ==> @eutt E' (prod (alist var value) R) (prod _ R) eq)
            interp_locals.
   Proof.
     repeat intro.
     unfold interp_locals.
-    unfold run_env.
+    unfold run_map.
     rewrite H0. eapply eutt_interp_state; auto.
     rewrite H; reflexivity.
   Qed.
 
+  (** [interp_locals] commutes with [bind]. *)
   Lemma interp_locals_bind: forall {R S} (t: itree E R) (k: R -> itree _ S) (s: alist var value),
       @eutt E' _ _ eq
             (interp_locals (ITree.bind t k) s)
@@ -207,22 +347,36 @@ Section Correctness.
   Proof.
     intros.
     unfold interp_locals.
-    unfold run_env.
+    unfold run_map.
     rewrite interp_bind.
     rewrite interp_state_bind.
     reflexivity.
   Qed.
 
+  (** Definition of our bisimulation relation.
+      As previously explained, it relates up-to-tau two [itree]s after having
+      interpreted their [Locals] event.
+      We additionally bake into it a simulation relation taken in parameter:
+      - Local events are interpreted from related states.
+      - Returned values must contain related states, as well as computed datas
+      related by another relation [RR] taken in parameter.
+      In our case, we specialize [RR] to equality since both trees return [unit],
+      and [Renv_] to [Renv].
+   *)
+  (* SAZ: TODO - rename some of the variables here to make it clear what are environemnts, etc. 
+     maybe rename a and b to use pattern binding: a == '(src_env, src_res)
+  *)
   Definition eq_locals {R1 R2} (RR : R1 -> R2 -> Prop)
              (Renv_ : _ -> _ -> Prop)
-             t1 t2 :=
+             (t1: itree E R1) (t2: itree E R2): Prop :=
     forall g1 g2,
       Renv_ g1 g2 ->
       eutt (fun a (b : alist var value * R2) => Renv_ (fst a) (fst b) /\ RR (snd a) (snd b))
            (interp_locals t1 g1)
            (interp_locals t2 g2).
 
-  Instance eutt_eq_locals (Renv_ : _ -> _ -> Prop) {R} RR :
+  (** [eq_locals] is compatible with [eutt]. *)
+  Global Instance eutt_eq_locals (Renv_ : _ -> _ -> Prop) {R} RR :
     Proper (eutt eq ==> eutt eq ==> iff) (@eq_locals R R RR Renv_).
   Proof.
     repeat intro.
@@ -231,6 +385,7 @@ Section Correctness.
     - rewrite H, H0; auto.
   Qed.
 
+  (** [eq_locals] commutes with [bind]  *)
   Definition eq_locals_bind_gen (Renv_ : _ -> _ -> Prop)
              {R1 R2 S1 S2} (RR : R1 -> R2 -> Prop)
              (RS : S1 -> S2 -> Prop) :
@@ -247,207 +402,71 @@ Section Correctness.
     intros. eapply H0; destruct H2; auto.
   Qed.
 
+  (** [eq_locals] is compatible with [loop]. *)
   Lemma eq_locals_loop {A B C} x (t1 t2 : C + A -> itree E (C + B)) :
     (forall l, eq_locals eq Renv (t1 l) (t2 l)) ->
     eq_locals eq Renv (loop t1 x) (loop t2 x).
   Proof.
-    unfold eq_locals, interp_locals, run_env.
+    unfold eq_locals, interp_locals, run_map.
     intros. unfold loop.
     rewrite 2 interp_loop.
     eapply interp_state_loop; auto.
   Qed.
 
-  Ltac force_left :=
-    match goal with
-    | |- eutt _ ?x _ => rewrite (itree_eta x); cbn
-    end.
-
-  Ltac force_right :=
-    match goal with
-    | |- eutt _ _ ?x => rewrite (itree_eta x); cbn
-    end.
-
-  Ltac untau_left := force_left; rewrite tau_eutt.
-  Ltac untau_right := force_right; rewrite tau_eutt.
-
-
-  Notation "(% x )" := (gen_tmp x) (at level 1).
-
-  Lemma compile_expr_correct : forall e g_imp g_asm n,
-      Renv g_asm g_imp ->
-      eutt (sim_rel g_asm n)
-           (interp_locals (denote_list (compile_expr n e)) g_asm)
-           (interp_locals (denoteExpr e) g_imp).
+  (** [sim_rel] at [n] entails that [GetVar (gen_tmp n)] gets interpreted
+      as returning the same value as the _Imp_ related one.
+   *)
+  Lemma sim_rel_get_tmp0:
+    forall n g_asm0 g_asm g_imp v,
+      sim_rel g_asm0 n (g_asm,tt) (g_imp,v) ->
+      interp_locals (send (GetVar (gen_tmp n))) g_asm ≈ Ret (g_asm,v).
   Proof.
-    induction e; simpl; intros.
-    - repeat untau_left.
-      repeat untau_right.
-      force_left; force_right.
-      apply eutt_ret.
-      erewrite <- Renv_find; [| eassumption].
-      apply sim_rel_add; assumption.
-    - repeat untau_left.
-      force_left.
-      force_right.
-      apply eutt_ret.
-      apply sim_rel_add; assumption.
-    - do 2 setoid_rewrite denote_list_app.
-      do 2 setoid_rewrite interp_locals_bind.
-      eapply eutt_bind_gen.
-      + eapply IHe1; assumption.
-      + intros [g_asm' []] [g_imp' v] HSIM.
-        eapply eutt_bind_gen.
-        eapply IHe2.
-        eapply sim_rel_Renv; eassumption.
-        intros [g_asm'' []] [g_imp'' v'] HSIM'.
-        repeat untau_left.
-        force_left; force_right.
-        simpl fst in *.
-        (* TODO: Simplify this *)
-        apply eutt_ret.
-        {
-          generalize HSIM; intros LU; apply sim_rel_find_tmp_n in LU.
-          unfold alist_In in LU; erewrite sim_rel_find_tmp_lt_n in LU; eauto; fold (alist_In (%n) g_asm'' v) in LU.
-          generalize HSIM'; intros LU'; apply sim_rel_find_tmp_n in LU'.
-          rewrite LU,LU'.
-          split; [| split].
-          {
-            eapply Renv_add, sim_rel_Renv; eassumption.
-          }
-          {
-            apply In_add_eq.
-          }
-          {
-            intros m LT v''.
-            rewrite <- In_add_ineq_iff; [| apply gen_tmp_inj; lia].
-            destruct HSIM as [_ [_ HSIM]].
-            destruct HSIM' as [_ [_ HSIM']].
-            rewrite HSIM; [| auto with arith].
-            rewrite HSIM'; [| auto with arith].
-            reflexivity.
-          }
-        }
-    - do 2 setoid_rewrite denote_list_app.
-      do 2 setoid_rewrite interp_locals_bind.
-      eapply eutt_bind_gen.
-      + eapply IHe1; assumption.
-      + intros [g_asm' []] [g_imp' v] HSIM.
-        eapply eutt_bind_gen.
-        eapply IHe2.
-        eapply sim_rel_Renv; eassumption.
-        intros [g_asm'' []] [g_imp'' v'] HSIM'.
-        repeat untau_left.
-        force_left; force_right.
-        simpl fst in *.
-        (* TODO: Simplify this *)
-        apply eutt_ret.
-        {
-          generalize HSIM; intros LU; apply sim_rel_find_tmp_n in LU.
-          unfold alist_In in LU; erewrite sim_rel_find_tmp_lt_n in LU; eauto; fold (alist_In (%n) g_asm'' v) in LU.
-          generalize HSIM'; intros LU'; apply sim_rel_find_tmp_n in LU'.
-          rewrite LU,LU'.
-          split; [| split].
-          {
-            eapply Renv_add, sim_rel_Renv; eassumption.
-          }
-          {
-            apply In_add_eq.
-          }
-          {
-            intros m LT v''.
-            rewrite <- In_add_ineq_iff; [| apply gen_tmp_inj; lia].
-            destruct HSIM as [_ [_ HSIM]].
-            destruct HSIM' as [_ [_ HSIM']].
-            rewrite HSIM; [| auto with arith].
-            rewrite HSIM'; [| auto with arith].
-            reflexivity.
-          }
-        }
-    - do 2 setoid_rewrite denote_list_app.
-      do 2 setoid_rewrite interp_locals_bind.
-      eapply eutt_bind_gen.
-      + eapply IHe1; assumption.
-      + intros [g_asm' []] [g_imp' v] HSIM.
-        eapply eutt_bind_gen.
-        eapply IHe2.
-        eapply sim_rel_Renv; eassumption.
-        intros [g_asm'' []] [g_imp'' v'] HSIM'.
-        repeat untau_left.
-        force_left; force_right.
-        simpl fst in *.
-        (* TODO: Simplify this *)
-        apply eutt_ret.
-        {
-          generalize HSIM; intros LU; apply sim_rel_find_tmp_n in LU.
-          unfold alist_In in LU; erewrite sim_rel_find_tmp_lt_n in LU; eauto; fold (alist_In (%n) g_asm'' v) in LU.
-          generalize HSIM'; intros LU'; apply sim_rel_find_tmp_n in LU'.
-          rewrite LU,LU'.
-          split; [| split].
-          {
-            eapply Renv_add, sim_rel_Renv; eassumption.
-          }
-          {
-            apply In_add_eq.
-          }
-          {
-            intros m LT v''.
-            rewrite <- In_add_ineq_iff; [| apply gen_tmp_inj; lia].
-            destruct HSIM as [_ [_ HSIM]].
-            destruct HSIM' as [_ [_ HSIM']].
-            rewrite HSIM; [| auto with arith].
-            rewrite HSIM'; [| auto with arith].
-            reflexivity.
-          }
-        }
-  Qed.
-
-  Lemma compile_assign_correct : forall e x,
-      eq_locals eq Renv
-                (denote_list (compile_assign x e))
-                (v <- denoteExpr e ;; lift (SetVar x v)).
-  Proof.
-    red; intros.
-    unfold compile_assign.
-    rewrite denote_list_app.
-    do 2 rewrite interp_locals_bind.
-    eapply eutt_bind_gen.
-    eapply compile_expr_correct; eauto.
     intros.
-    repeat untau_left.
-    force_left.
-    repeat untau_right; force_right.
-    eapply eutt_ret; simpl.
-    destruct r1, r2.
-    erewrite sim_rel_find_tmp_n; eauto; simpl.
-    destruct H0.
-    split; auto.
-    eapply Renv_write_local; eauto.
+    destruct H as [_ [eq _]].
+    unfold interp_locals.
+    unfold send.
+    rewrite interp_send.
+    rewrite tau_eutt.
+    cbn.
+    unfold run_map.
+    unfold evalLocals, CategoryOps.cat, Cat_Handler, Handler.cat.
+    unfold lookup_def; cbn.
+    rewrite unfold_interp_state; cbn.
+    rewrite tau_eutt.
+    rewrite map_bind.
+    setoid_rewrite bind_ret.
+    setoid_rewrite interp_ret.
+    unfold inl_, Inl_sum1_Handler, Handler.inl_, Handler.hsend.
+    rewrite interp_state_bind.
+    rewrite interp_state_send.
+    cbn.
+    rewrite eq.
+    rewrite !tau_eutt.
+    rewrite bind_ret; cbn.
+    rewrite interp_state_ret.
+    reflexivity.
   Qed.
-Require Import Label.
-Instance eq_itree_loop_Label {E A B C} :
-  Proper ((eq ==> eq_itree eq) ==> eq ==> eq_itree eq) (@loop_Label E A B C).
-Proof.
-Admitted.
 
-Global Instance eq_lift_Label {A B} :
-  Proper (eq2 ==> eq2) (@lift_Label E A B).
-Proof.
-Admitted.
-Instance sutt_loop_Label {E A B C} :
-  Proper (pointwise_relation _ (sutt eq) ==> eq ==> sutt eq) (@loop_Label E A B C).
-Proof.
-Admitted.
+End Eq_Locals.
 
-Instance eutt_loop_Label {E A B C} :
-  Proper (pointwise_relation _ (eutt eq) ==> eq ==> eutt eq) (@loop_Label E A B C).
-  Admitted.
+(* ================================================================= *)
+(** ** Linking *)
 
-Global Instance eq_ktree_loop_Label {I A B} :
-  Proper (eq2 ==> eq2) (@loop_Label E I A B).
-Proof.
-Admitted.
+(** We first show that our "high level" [asm] combinators are correct.
+    These proofs are mostly independent from the compiler, and therefore
+    fairly reusable.
+    Once again, these notion of correctness are expressed as equations
+    commuting the denotation with the combinator.
+ *)
 
+Section Linking.
 
+  Context {E': Type -> Type}.
+  Context {HasMemory: Memory -< E'}.
+  Context {HasExit: Exit -< E'}.
+  Notation E := (Locals +' E').
+(*
+  (** [seq_asm] is denoted as the (horizontal) composition of denotations. *)
   Lemma seq_asm_correct {A B C} (ab : asm A B) (bc : asm B C) :
       denote_asm (seq_asm ab bc)
     ⩯ denote_asm ab >>> denote_asm bc.
@@ -455,21 +474,21 @@ Admitted.
     unfold seq_asm. 
     rewrite link_asm_correct, relabel_asm_correct, app_asm_correct.
     rewrite <- lift_ktree_id, cat_assoc.
-    (* rewrite cat_id_r. *)
-    (* rewrite sym_ktree_unfold. *)
-    (* apply cat_from_loop. *)
-    (* all: typeclasses eauto. *)
-  (* Qed. *)
-  Admitted.
+    rewrite cat_id_r.
+    rewrite sym_ktree_unfold.
+    apply cat_from_loop.
+    all: typeclasses eauto.
+  Qed.
 
-  Lemma if_asm_correct {A} (e : list instr) (tp fp : asm 1 A) :
+  (** [if_asm] is denoted as the ktree first denoting the branching condition,
+      then looking-up the appropriate variable and following with either denotation. *)
+  Lemma if_asm_correct {A} (e : list instr) (tp fp : asm unit A) :
       denote_asm (if_asm e tp fp)
     ⩯ ((fun _ =>
          denote_list e ;;
-                     v <- lift (GetVar tmp_if) ;;
-                     if v : value then denote_asm fp F1 else denote_asm tp F1) : ktree _ _ _).
+         v <- send (GetVar tmp_if) ;;
+         if v : value then denote_asm fp tt else denote_asm tp tt) : ktree _ _ _).
   Proof.
-(*
     unfold if_asm.
     rewrite seq_asm_correct.
     unfold cond_asm.
@@ -503,16 +522,16 @@ Admitted.
       unfold inl_, Inl_ktree, lift_ktree;
         rewrite bind_ret_; reflexivity.
   Qed.
- *)
-  Admitted.
 
-  Lemma while_asm_correct (e : list instr) (p : asm 1 1) :
+  (** [while_asm] is denoted as the loop of the body with two entry point, the exit
+      of the loop, and the body in which we have the same structure as for the conditional *)
+   Lemma while_asm_correct (e : list instr) (p : asm unit unit) :
       denote_asm (while_asm e p)
-    ⩯ loop_Label (fun l : unit + unit =>
+    ⩯ loop (fun l : unit + unit =>
          match l with
          | inl tt =>
            denote_list e ;;
-           v <- ITree.lift (inl1 (GetVar tmp_if)) ;;
+           v <- ITree.send (inl1 (GetVar tmp_if)) ;;
            if v : value then
              Ret (inr tt)
            else
@@ -522,11 +541,7 @@ Admitted.
   Proof.
     unfold while_asm.
     rewrite link_asm_correct.
-    (* TODO: this is a hack it should just be
-     apply eq_ktree_loop. *)
-    match goal with
-    | [ |- _ (loop ?x) (loop ?y) ] => apply (eq_ktree_loop x y)
-    end.
+    apply eq_ktree_loop.
     rewrite relabel_asm_correct.
     rewrite <- lift_ktree_id, cat_id_l.
     rewrite app_asm_correct.
@@ -551,156 +566,371 @@ Admitted.
         repeat rewrite bind_ret_; reflexivity.
     - rewrite itree_eta; cbn; reflexivity.
   Qed.
+*)
+End Linking.
 
+(* ================================================================= *)
+(** ** Correctness *)
+
+Section Correctness.
+
+  Context {E': Type -> Type}.
+  Context {HasMemory: Memory -< E'}.
+  Context {HasExit: Exit -< E'}.
+  Notation E := (Locals +' E').
+
+  (** We use a couple of tactics to step through itrees by eta expansion followed by reduction *)
+  Ltac force_left :=
+    match goal with
+    | |- eutt _ ?x _ => rewrite (itree_eta x); cbn
+    end.
+
+  Ltac force_right :=
+    match goal with
+    | |- eutt _ _ ?x => rewrite (itree_eta x); cbn
+    end.
+
+  (** Chain a reduction expected to exhibit a [Tau] step with its elimination *)
+  Ltac untau_left := force_left; rewrite tau_eutt.
+  Ltac untau_right := force_right; rewrite tau_eutt.
+
+  (** Fully reduce both sides *)
+  Ltac tau_steps :=
+    repeat (untau_left); force_left;
+    repeat (untau_right); force_right.
+
+  (** Correctness of expressions.
+      We strengthen [eq_locals]: initial environments are still related by [Renv],
+      but intermediate ones must now satisfy [sim_rel].
+      Note that by doing so, we use a _heterogeneous bisimulation_: the trees
+      return values of different types ([alist var value * unit] for _Asm_,
+      [alist var value * value] for _Imp_). The differeence is nonetheless mostly
+      transparent for the user, except for the use of the more generale [eutt_bind_gen].
+   *)
+  
+  Lemma compile_expr_correct : forall e g_imp g_asm n,
+      Renv g_asm g_imp ->
+      eutt (sim_rel g_asm n)
+           (interp_locals (denote_list (compile_expr n e)) g_asm)
+           (interp_locals (denoteExpr e) g_imp).
+  Proof.
+    induction e; simpl; intros.
+    - (* Var case *)
+      (* We first compute and eliminate taus on both sides. *)
+      tau_steps.
+
+      (* We are left with [Ret] constructs on both sides, that remains to be related *)
+      apply eutt_ret.
+      (* On the _Asm_ side, we bind to [gen_tmp n] a lookup to [varOf v] *)
+      (* On the _Imp_ side, we return the value of a lookup to [varOf v] *)
+      erewrite <- Renv_find; [| eassumption].
+      apply sim_rel_add; assumption.
+
+    - (* Literal case *)
+      (* We reduce both sides to Ret constructs *)
+      tau_steps.
+
+      apply eutt_ret.
+      (* _Asm_ bind the litteral to [gen_tmp n] while _Imp_ returns it *)
+      apply sim_rel_add; assumption.
+
+    (* The three binary operator cases are identical *)
+    - (* Plus case *)
+      (* We push [interp_locals] into the denotations *)
+      do 2 setoid_rewrite denote_list_app.
+      do 2 setoid_rewrite interp_locals_bind.
+
+      (* The Induction hypothesis on [e1] relates the first itrees *)
+      eapply eutt_bind_gen.
+      { eapply IHe1; assumption. }
+      (* We obtain new related environments *)
+      intros [g_asm' []] [g_imp' v] HSIM.
+      (* The Induction hypothesis on [e2] relates the second itrees *)
+      eapply eutt_bind_gen.
+      { eapply IHe2.
+        eapply sim_rel_Renv; eassumption. }
+      (* And we once again get new related environments *)
+      intros [g_asm'' []] [g_imp'' v'] HSIM'.
+      (* We can now reduce down to Ret constructs that remains to be related *)
+      tau_steps.
+      simpl fst in *.
+      apply eutt_ret.
+
+      clear -HSIM HSIM'.
+      erewrite sim_rel_find_tmp_n_trans; eauto. 
+      erewrite sim_rel_find_tmp_n; eauto. 
+      eapply sim_rel_binary_op; eauto.
+
+    - (* Sub case *)
+      (* We push [interp_locals] into the denotations *)
+      do 2 setoid_rewrite denote_list_app.
+      do 2 setoid_rewrite interp_locals_bind.
+
+      (* The Induction hypothesis on [e1] relates the first itrees *)
+      eapply eutt_bind_gen.
+      { eapply IHe1; assumption. }
+      (* We obtain new related environments *)
+      intros [g_asm' []] [g_imp' v] HSIM.
+      (* The Induction hypothesis on [e2] relates the second itrees *)
+      eapply eutt_bind_gen.
+      { eapply IHe2.
+        eapply sim_rel_Renv; eassumption. }
+      (* And we once again get new related environments *)
+      intros [g_asm'' []] [g_imp'' v'] HSIM'.
+      (* We can now reduce down to Ret constructs that remains to be related *)
+      tau_steps. 
+      simpl fst in *.
+      apply eutt_ret.
+
+      clear -HSIM HSIM'.
+      erewrite sim_rel_find_tmp_n_trans; eauto. 
+      erewrite sim_rel_find_tmp_n; eauto. 
+      eapply sim_rel_binary_op; eauto.
+
+    - (* Mul case *)
+      (* We push [interp_locals] into the denotations *)
+      do 2 setoid_rewrite denote_list_app.
+      do 2 setoid_rewrite interp_locals_bind.
+
+      (* The Induction hypothesis on [e1] relates the first itrees *)
+      eapply eutt_bind_gen.
+      { eapply IHe1; assumption. }
+      (* We obtain new related environments *)
+      intros [g_asm' []] [g_imp' v] HSIM.
+      (* The Induction hypothesis on [e2] relates the second itrees *)
+      eapply eutt_bind_gen.
+      { eapply IHe2.
+        eapply sim_rel_Renv; eassumption. }
+      (* And we once again get new related environments *)
+      intros [g_asm'' []] [g_imp'' v'] HSIM'.
+      (* We can now reduce down to Ret constructs that remains to be related *)
+      tau_steps.
+      simpl fst in *.
+      apply eutt_ret.
+
+      clear -HSIM HSIM'.
+      erewrite sim_rel_find_tmp_n_trans; eauto. 
+      erewrite sim_rel_find_tmp_n; eauto. 
+      eapply sim_rel_binary_op; eauto.
+  Qed.
+
+  (** Correctness of the assign statement.
+      The resulting list of instruction is denoted as
+      denoting the expression followed by setting the variable.
+   *)
+  Lemma compile_assign_correct : forall e x,
+      eq_locals eq Renv
+                (denote_list (compile_assign x e))
+                (v <- denoteExpr e ;; send (SetVar x v)).
+  Proof.
+    red; intros.
+    unfold compile_assign.
+    (* We push interp_locals inside of the denotations *)
+    rewrite denote_list_app.
+    do 2 rewrite interp_locals_bind.
+
+    (* By correctness of the compilation of expressions,
+       we can match the head trees.
+     *)
+    eapply eutt_bind_gen.
+    { eapply compile_expr_correct; eauto. }
+
+    (* Once again, we get related environments *)
+    intros [g_asm' []] [g_imp' v] HSIM.
+    (* We can now reduce to Ret constructs *)
+    tau_steps. 
+    eapply eutt_ret; simpl.
+
+    (* And remains to relate the results *)
+    erewrite sim_rel_find_tmp_n; eauto; simpl.
+    apply sim_rel_Renv in HSIM.
+    split; auto.
+    eapply Renv_write_local; eauto.
+  Qed.
+
+  (* Utility: slight rephrasing of [while] to facilitate rewriting
+     in the main theorem.*)
   Lemma while_is_loop {E} (body : itree E bool) :
     while body
           ≈ loop (fun l : unit + unit =>
                     match l with
-                    | inl _ => ITree.map (fun b => if b : bool then inl tt else inr tt)
-                                        body
+                    | inl _ => ITree.map (fun b => if b : bool then inl tt else inr tt) body
                     | inr _ => Ret (inl tt)   (* Enter loop *)
                     end) tt.
   Proof.
     unfold while.
-    (* another hack, should be [apply eutt_loop]. *)
-    match goal with
-    | [ |- _ (loop ?x _) (loop ?y _) ] =>
-    apply (eutt_loop x y)
-    end;
-      [intros [[]|[]]; simpl |]; try reflexivity.
+    apply eutt_loop; [| reflexivity].
+    intros [[]|[]]; simpl; [| reflexivity].
     unfold ITree.map.
     apply eutt_bind; try reflexivity.
     intros []; reflexivity.
   Qed.
 
-  Definition env_lookupDefault_is_lift {K V : Type} {E: Type -> Type} `{envE K V -< E} (x: K) (v: V):
-    env_lookupDefault x v = lift (lookupDefaultE x v).
-  Proof.
-    reflexivity.
-  Qed.
-
-  Lemma sim_rel_get_tmp0:
-    forall g_asm0 g_asm g_imp v,
-      sim_rel g_asm0 0 (g_asm,tt) (g_imp,v) ->
-      interp_locals (lift (GetVar (%0))) g_asm ≈ Ret (g_asm,v).
-  Proof.
-    intros.
-    destruct H as [_ [eq _]].
-    unfold interp_locals.
-    unfold lift.
-    rewrite interp_lift.
-    rewrite tau_eutt.
-    cbn.
-    unfold run_env.
-    unfold evalLocals, CategoryOps.cat, Cat_Handler, Handler.cat.
-    rewrite env_lookupDefault_is_lift.
-    unfold lift.
-    rewrite unfold_interp_state; cbn.
-    rewrite tau_eutt.
-    rewrite map_bind.
-    setoid_rewrite interp_ret.
-    setoid_rewrite bind_ret2.
-    unfold inl_, Inl_sum1_Handler, Handler.inl_, Handler.hlift.
-    rewrite interp_state_lift.
-    rewrite bind_ret2.
-    cbn.
-    rewrite eq.
-    rewrite !tau_eutt.
-    reflexivity.
-  Qed.
-
-  Lemma compile_correct (s : stmt) :
+  (*
+  (** Correctness of the compiler.
+      After interpretation of the [Locals], the source _Imp_ statement
+      denoted as an [itree] and the compiled _Asm_ program denoted
+      as an [itree] are equivalent up-to-taus.
+      The correctness is termination sensitive, but nonetheless a simple
+      induction on statements.
+      We only are left with reasoning about the functional correctness of
+      the compiler, all control-flow related reasoning having been handled
+      in isolation.
+   *)
+  Theorem compile_correct (s : stmt) :
     eq_locals eq Renv
-              (denote_asm (compile s) tt)
+              (denote_asm (compile s) Fin.F1)
               (denoteStmt s).
   Proof.
     induction s.
 
     - (* Assign *)
       simpl.
+      (* We push [denote_asm] inside of the combinators *)
       rewrite raw_asm_block_correct.
       rewrite after_correct.
+
+      (* The head trees match by correctness of assign *)
       rewrite <- (bind_ret2 (ITree.bind (denoteExpr e) _)).
       eapply eq_locals_bind_gen.
       { eapply compile_assign_correct; auto. }
-      intros [] [] []. simpl.
+
+      (* And remains to trivially relate the results *)
+      intros [] [] []; simpl.
       repeat intro.
-      rewrite itree_eta, (itree_eta (_ _ g2)); cbn.
+      force_left; force_right.
       apply eutt_ret; auto.
 
     - (* Seq *)
+      (* We commute [denote_asm] with [seq_asm] *)
       rewrite fold_to_itree; simpl.
       rewrite seq_asm_correct. unfold to_itree.
-      unfold ITree.cat.
+
+      (* And the result is immediate by indcution hypothesis *)
       eapply eq_locals_bind_gen.
       { eauto. }
       intros [] [] []; auto.
 
     - (* If *)
-      repeat intro.
+      (* We commute [denote_asm] with [if_asm] *)
       rewrite fold_to_itree. simpl.
       rewrite if_asm_correct.
       unfold to_itree.
+
+      (* We now need to line up the evaluation of the test,
+         and eliminate them by correctness of [compile_expr] *)
+      repeat intro.
       rewrite 2 interp_locals_bind.
       eapply eutt_bind_gen.
       { apply compile_expr_correct; auto. }
-      intros.
-      destruct r2 as [g_imp' v]; simpl.
+
+      (* We get in return [sim_rel] related environments *)
+      intros [g_asm []] [g_imp v] HSIM.
       rewrite interp_locals_bind.
-      destruct r1 as [g_asm' []].
-      generalize H0; intros EQ. apply sim_rel_get_tmp0 in EQ.
+      (* We know that interpreting [GetVar tmp_if] is eutt to [Ret (g_asm,v)] *)
+      generalize HSIM; intros EQ; eapply sim_rel_get_tmp0 in EQ.
       setoid_rewrite EQ; clear EQ.
-      rewrite bind_ret_.
-      simpl.
-      apply sim_rel_Renv in H0.
+      rewrite bind_ret_; simpl.
+      (* We can weaken [sim_rel] down to [Renv] *)
+      apply sim_rel_Renv in HSIM.
+      (* And finally conclude in both cases *)
       destruct v; simpl; auto. 
 
     - (* While *)
+      (* We commute [denote_asm] with [while_asm], and restructure the
+         _Imp_ [loop] with [while_is_loop] *)
       simpl; rewrite fold_to_itree.
       rewrite while_asm_correct.
       rewrite while_is_loop.
       unfold to_itree.
-      (* TODO: [apply eq_locals_loop] *)
-      match goal with
-      | [ |- _ (loop ?x _) (loop ?y _) ] =>
-        apply (eq_locals_loop _ x y)
-      end.
-      intros [[]|[]].
-      2:{ repeat intro.
-          rewrite itree_eta, (itree_eta (_ _ g2)); cbn.
-          apply eutt_ret; auto. }
-      unfold ITree.map. rewrite bind_bind.
 
+      (* We now have loops on both side, so we can just reason about their bodies *)
+      apply eq_locals_loop.
+      (* The two cases correspond to entering the loop, or exiting it*)
+      intros [[]|[]].
+
+      (* The exiting case is trivial *)
+      2:{ repeat intro.
+          force_left. force_right.
+          apply eutt_ret; auto. }
+
+      (* We now need to line up the evaluation of the test,
+         and eliminate them by correctness of [compile_expr] *)
+      unfold ITree.map. rewrite bind_bind.
       repeat intro.
       rewrite 2 interp_locals_bind.
       eapply eutt_bind_gen.
       { apply compile_expr_correct; auto. }
-      intros.
-      destruct r2 as [g_imp' v]; simpl.
-      rewrite interp_locals_bind.
-      destruct r1 as [g_asm' []].
-      generalize H0; intros EQ. apply sim_rel_get_tmp0 in EQ.
-      rewrite interp_locals_bind.
+
+      (* We get in return [sim_rel] related environments *)
+      intros [g_asm []] [g_imp v] HSIM.
+      rewrite 2 interp_locals_bind.
+      (* We know that interpreting [GetVar tmp_if] is eutt to [Ret (g_asm,v)] *)
+      generalize HSIM; intros EQ. eapply sim_rel_get_tmp0 in EQ.
       setoid_rewrite EQ; clear EQ.
-      rewrite bind_ret_.
-      simpl.
-      apply sim_rel_Renv in H0.
+      rewrite bind_ret_; simpl.
+
+      (* We can weaken [sim_rel] down to [Renv] *)
+      apply sim_rel_Renv in HSIM.
+      (* And now consider both cases *)
       destruct v; simpl; auto.
-      + rewrite itree_eta, (itree_eta (_ >>= _)); cbn.
-        apply eutt_ret. auto.
-      + rewrite 2 interp_locals_bind, bind_bind.
+      + (* The false case is trivial *)
+        force_left; force_right.
+        apply eutt_ret; auto.
+      + (* In the true case, we line up the body of the loop to use the induction hypothesis *)
+        rewrite 2 interp_locals_bind, bind_bind.
         eapply eutt_bind_gen.
         { eapply IHs; auto. }
+        intros [g_asm' []] [g_imp' v'] [HSIM' ?].
         intros.
-        rewrite itree_eta, (itree_eta (_ >>= _)); cbn.
-        apply eutt_ret. destruct H1; auto.
+        force_right; force_left.
+        apply eutt_ret; simpl; split; auto. 
 
     - (* Skip *)
       repeat intro.
-      rewrite (itree_eta (_ (denote_asm _ _) _)),
-      (itree_eta (_ (denoteStmt _) _));
-        cbn.
+      force_right; force_left.
       apply eutt_ret; auto.
   Qed.
-
+*)
 End Correctness.
+
+(* ================================================================= *)
+(** ** Closing word. *)
+
+(** Through this medium-sized exemple, we have seen how to use [itree]s to
+    denote two languages, how to run them and how to prove correct a compiler
+    between them both.
+    We have emphasized that the theory of [ktree]s allowed us to decouple
+    all reasoning about the control-flow from the proof of the compiler itself.
+    The resulting proof is entirely structurally inductive and equational. In
+    particular, we obtain a final theorem relating potentially infinite computations
+    without having to write any cofixpoint. 
+    
+    If this result is encouraging, one might always wonder how things scale.
+
+    A first good sanity check is to extend the languages with a _Print_ instruction.
+    It requires to add a new effect to the language and therefore makes the correctness
+    theorem relate trees actually still containing events.
+    This change, which a good exercise to try, turns out to be as straightforward as one
+    would hope. The only new lemma needed is to show that [interp_locals] leaves the
+    new [Print] effect untouched.
+    This extension can be found in the _tutorial-print_ branch.
+
+    More importantly, our compiler is fairly stupid and inefficient: it creates blocks
+    for each compiled statement! One would hope to easily write and prove an optimization
+    coalescing elementary blocks together.
+    This however raises for now a difficulty: our representation of labels as binary trees
+    encoded in [Type] is so unstructured that introspection on [asm] programs is difficult.
+    We might therefore need to change our representation of labels, for instance to a [Fin] type.
+    But this change turns out to be more interesting that it might seem: it moves [bks]
+    from [fun (A B: Type) => A -> block B] to [fun (A B: nat) => Fin.t A -> block (Fin.t B)].
+    Correspondingly, their denotation moves from [fun (A B: Type) => bks A B -> ktree E A B]
+    to [fun (A B: nat) => ktree E (Fin.t A) (Fin.t B)].
+    But our proof crucially rested on the categorie [(Type, ktree E)] being provided by
+    the [itree] library with a traced monoidal structure. We would therefore here need
+    to redo all the work to equip the category [(Nat, fun A B => ktree E (t A) (t B))] with
+    the same strucutre, which is significant low level work.
+    We might therefore want to investigate whether [ktree] should be generalized to 
+    something along the lines of
+    [ktree (i : Type) (F : i -> Type) (E : Type -> Type) (a b : i) : Type := F a -> itree E (F b).]
+ *)
